q

qr.ec
@@ -1,5 +1,5 @@
 pragma Goals:printall.
-require import AllCore DBool Bool.
+require import AllCore DBool Bool List.
 
 
 (*
@@ -40,6 +40,13 @@ skip. progress;smt.
 qed.
 
 
+lemma exp_lemmaaa : equiv[ Exp.main1 ~ Exp.main2 : true ==> ={res} /\ (res{2}.`2 = false => res{1}.`1 = res{2}.`1) ].
+proof. proc. swap 1 1.
+rnd (fun x => x ^^ Exp.b2{1}). rnd. 
+skip. progress;smt.
+qed.
+
+
 
 
 
@@ -55,8 +62,17 @@ module type Verifier = {
 }.
 
 
+
+module type VerifierA = {
+  proc challenge(N : int, y : int, c : int) : bool  
+  proc summitup(c : int, b : bool, r : int) : bool list
+}.
+
+
+
+
 module type Simulator = {
-  proc simulate(N : int, y : int) : int * bool * int * bool
+  proc simulate(N : int, y : int) : bool list
 }.
 
 
@@ -69,31 +85,32 @@ module QRP(P : Prover, V : Verifier) = {
     c <- P.commit(N, y);  
     b <- V.challenge(N,y,c);
     r <- P.response(b);
-    result <- V.verify(c,b,r);
+    result <- V.verify(c,b,r);  (*  *)
     return result;
   }
 }.
 
 
 
-op zn :  int -> int distr.
-op qr : int -> int -> int option.
+op sqDist :  int -> int distr.
+op sqRoot : int -> int -> int.
 
-axiom qr_prop1 (Na ya z : int) : qr Na ya = Some z => z * z = ya.
-axiom qr_prop2 (Na ya z : int) : z * z = ya => qr Na ya = Some z.
+
+axiom qr_prop1 (Na ya z : int) : sqRoot Na ya = z => z * z = ya.
+axiom qr_prop2 (Na ya z : int) : z * z = ya => sqRoot Na ya = z.
 
 
 module HP : Prover = {
-  var z, n, y : int
+  var rr, n, y : int
 
   proc commit(n1 : int, y1 : int) : int = {  
     (n,y) <- (n1, y1);
-    z <$ zn n;
-    return z*z;
+    rr <$ sqDist n;
+    return rr;
   }
 
   proc response(b : bool) : int = {
-    return z * (if b then (oget (qr n y)) else 1);
+    return (sqRoot n rr) * (if b then (sqRoot n y) else 1);
  } 
 }.
 
@@ -116,11 +133,11 @@ module HV : Verifier = {
 
 
 lemma qrp_complt Na ya z :
- qr Na ya = Some z => hoare [ QRP(HP,HV).main : arg = (Na,ya) ==> res  ].
+ sqRoot Na ya =  z => hoare [ QRP(HP,HV).main : arg = (Na,ya) ==> res  ].
 proof. move => qra.
 proc.  inline*.  wp. 
 rnd. wp.  rnd.  wp. 
-skip. progress. rewrite qra. simplify.
+skip. progress. rewrite qra. simplify. smt.
 (* smt. *)
 admit.
 qed.
@@ -131,7 +148,7 @@ section.
 declare module P : Prover.
 
 lemma qrp_sound Na ya :
- qr Na ya = None => phoare [ QRP(P,HV).main : arg = (Na,ya) ==> res ] = (1%r/2%r).
+ sqRoot Na ya = 0 => phoare [ QRP(P,HV).main : arg = (Na,ya) ==> res ] = (1%r/2%r).
 proof. move => qra.
 proc. inline*. swap 6 -5.
 admitted. 
@@ -142,16 +159,258 @@ end section.
 
 section.
 
-declare module V : Verifier.
+declare module V : VerifierA {HP}.
 
-module Sim : Simulator = {
-  proc simulate(n : int, y : int) : int * bool * int * bool = {
-    return witness;
+
+
+(*
+?? transcript := network messages AND internal states
+
+Defs:
+- ZK wrt. transcript
+- ZK wrt. transcript + output bitstring
+- ZK wrt. output bitstring
+
+All equiv.
+
+*)
+
+
+
+local module Inits = {
+    
+  proc init1(N : int, y : int) = {
+    var z,c,b;
+    b <$ {0,1};
+    z  <$ sqDist N;    
+    c  <- z * if b then y else 1;
+    return (b, z);
+  }
+
+  proc init1_t(N : int, y : int) = {
+    var z,c;
+    z  <$ sqDist N;    
+    c  <- z * if true then y else 1;
+    return (true, c);
+  }
+
+  proc init1_f(N : int, y : int) = {
+    var z,c;
+    z  <$ sqDist N;    
+    c  <- z * if false then y else 1;
+    return (false, c);
+  }
+  
+  
+  proc init2(N : int, y : int) = {
+    var z,b;
+    b <$ {0,1};
+    z  <$ sqDist N;    
+    return (b, z);
+  }  
+
+  proc init2_t(N : int, y : int) = {
+    var z;
+    z  <$ sqDist N;    
+    return (true, z);
+  }    
+
+  proc init2_f(N : int, y : int) = {
+    var z;
+    z  <$ sqDist N;    
+    return (false, z);
+  }    
+  
+}.
+
+
+local lemma init_lemma_f :
+ equiv[ Inits.init1_f ~ Inits.init2_f : ={arg} ==> ={res} ].
+proof. proc. simplify.
+wp.
+rnd.
+skip. progress;smt.
+qed.
+
+
+op inv : int -> int -> int.
+local lemma init_lemma_t :
+ equiv[ Inits.init1_t ~ Inits.init2_t : ={arg} ==> ={res} ].
+proof. proc. simplify.
+wp. simplify.
+rnd (fun x => x * y{1}) (fun x => x * (inv N{1} y{1})). 
+skip. progress;admit.
+qed.
+
+
+
+
+local module Sim1  = {
+  var result : bool list
+
+
+
+  proc sinit(N : int, y : int) : bool * int * int = {
+    var rr,bb,zz;
+    bb <$ {0,1};
+    rr  <$ sqDist N;    
+    zz  <- rr * if bb then (inv N y) else 1;
+    return (bb,zz,rr);
+  }
+
+  proc simulate(N : int, y : int) : bool * bool list  = {
+    var rr,z,b',b,ryb;
+
+    (b',z,rr) <- sinit(N,y);
+    b  <- V.challenge(N,y,z);
+   
+
+    ryb  <- (sqRoot N rr);
+    result <- V.summitup(z,b,ryb); 
+    return (b = b', result);    
   }
 }.
 
 
-lemma qrp_zk Na ya : equiv [QRP(HP, V).main ~ Sim.simulate : ={arg} /\ arg{1} = (Na, ya) ==> 
-  (QRP.c,QRP.b,QRP.r, QRP.result){1} = res{2} ].
+
+
+local module Sim1'  = {
+  var result : bool list
+
+  proc sinit(N : int, y : int) : bool * int = {
+    var rr,bb;
+    rr  <$ sqDist N;    
+    bb <$ {0,1};
+    return (bb,rr);
+  }
+    
+  proc simulate(N : int, y : int) : bool * bool list  = {
+    var z,b',b,ryb,result;
+  
+    (b',z) <- sinit(N,y);
+    
+    b  <- V.challenge(N,y,z);
+
+    ryb  <- (sqRoot N (z * (if b then y else 1)));
+    result <- V.summitup(z,b,ryb); 
+    return (b = b', result);
+  }
+}.
+
+
+local lemma exss Na ya : equiv[ Sim1.sinit ~ Sim1'.sinit : ={arg} /\ arg{1} = (Na,ya) ==> (res{1}.`1, res{1}.`2) = res{2} /\ (res{1}.`1 = true => res{1}.`2 = res{1}.`3 * (inv Na ya)) /\ (res{1}.`1 = false => res{1}.`2 = res{1}.`3 /\ res{1}.`2 = res{2}.`2)  ].
+proof. proc. swap {2} 1 1.
+seq 1 1 : (={N,y,bb} /\ (N{1},y{1}) = (Na,ya)). rnd. skip. auto.
+exists* bb{1}. elim*. progress.
+wp.
+
+case (bb_L = true).
+rnd  (fun x => x * (inv N{1} y{1})) (fun x => x * y{1}).  skip. progress.
+admit. admit.  admit. admit.
+progress. rnd. skip. progress . smt.
+qed.
+
+
+
+local lemma qkok Na ya P : 
+  equiv [ Sim1.simulate ~ Sim1'.simulate : ={arg, glob V} /\ (Na,ya) = (N{1},y{1}) ==> res{1}.`1 /\ P res{1}.`2 => res{2}.`1 /\ P res{2}.`2   ].
+proof. proc.
+
+seq 1 1 : (={N,y,glob V,b',z} /\ (b'{1} = true => z{1} = rr{1} * (inv Na ya)) /\ (b'{2} = false => z{1} = rr{1} /\ z{1} = z{2}) ).
+
+call (exss Na ya). skip. progress.
+
+seq 1 1 : (={b,N,y,glob V,b',z} /\ (b'{1} = true => z{1} = rr{1} * (inv Na ya)) /\ (b'{2} = false => z{1} = rr{1} /\ z{1} = z{2})).
+call (_:true). skip. progress.
+
+exists* b'{1}. elim*. progress.
+
+case (b'_L = true).
+exists* b{1}. elim*. progress.
+case (b_L = true).
+
+
+seq 1 1 : (={b,N,y,glob V,b',z,ryb} /\ (b'{1} = true => z{1} = rr{1} * (inv Na ya)) /\ (b'{2} = false => z{1} = rr{1} /\ z{1} = z{2})).
+wp. skip. progress. rewrite H. auto.
+
+  call (_:true). skip. progress.
+
+sp.
+
+
+
+seq 1 1 : ((b'_L = b'{1} /\ ={N, y, b', glob V}) /\ b'_L = true /\ rr{2} *  inv N{2} y{2} = rr{1} ).
+
+
+skip. progress. admit.
+admit.
+admit.
+admit.
+admit.
+sp.
+
+conseq (_:  z{1} = rr{1} * inv N{1} y{1} /\ b'{1} = true /\ ={N, y, b', glob V} /\ rr{2} * inv N{2} y{2} = rr{1} ==> _).
+smt.
+
+seq 1 1 : (z{1} = rr{1} * inv N{1} y{1} /\ b'{1} = true /\ ={N, y, b', b, glob V} /\ rr{2} * inv N{2} y{2} = rr{1}).
+call (_:true). skip. progress.
+
+
+module ZK(P : Prover, V : VerifierA) = {
+  proc main(N : int, y : int) = {
+    var c,b,r,result;
+    c <- P.commit(N, y);  
+    b <- V.challenge(N,y,c);
+    r <- P.response(b);
+    result <- V.summitup(c,b,r); 
+    return result;
+  }
+}.
+
+
+
+local lemma qrp_zk2_eq Na ya : equiv [ZK(HP, V).main ~ Sim1'.simulate
+    : ={arg, glob V} /\ arg{1} = (Na, ya) ==> 
+        res{1} = res{2}.`2 ].
+proc.
+inline*. sp.
+call (_:true).
+wp. call (_:true).
+wp. swap {2} 2 -1.
+rnd. rnd {2}. skip. progress.
+qed.
+
+
+local lemma qrp_zk2_pr &m Na ya a :
+    Pr[ZK(HP, V).main(Na,ya) @ &m : res = a ] 
+     = Pr[ Sim1'.simulate(Na,ya) @ &m : res.`2 = a ].
+proof. byequiv.
+conseq (_: _ ==> res{1} = res{2}.`2 ). progress.
+conseq (qrp_zk2_eq Na ya). auto. auto. auto.
+qed.
+
+
+
+
+
+
+local lemma qrp_zk Na ya : equiv [ZK(HP, V).main ~ Sim1.simulate : ={arg} /\ arg{1} = (Na, ya) ==> 
+  ={res} ].
+proof.
+proc.  inline*.
+admitted.
+
+
+
+
+
+(* rewinds Sim1 N times *)
+local module SimN = {
+
+
+    
+}.
+
 
 end section.
+
