while.ec
@@ -1,0 +1,189 @@
+pragma Goals:printall.
+
+require import AllCore DBool.
+
+require import Int.
+print Int.
+op myd : int distr.
+
+module M = {
+
+  proc whp(c : int, n : int, b : bool, r : int) = {
+    while(c <= n /\ !b ){
+     r <$ myd;
+     b <$ {0,1};
+     c <- c + 1;
+    }
+    return (r,b);
+  }
+
+  proc main'_split(na : int) = {
+    var result,ba,ca;
+    result <- witness;
+    ba <- false;
+    ca <- 1;
+    if(ca <= na /\ !ba ){
+     result <$ myd;
+     ba <$ {0,1};
+     ca <- ca + 1;
+    }
+    (result,ba) <- whp(2,na,ba,result);
+    return result;
+  }
+
+
+  
+  proc main'(na : int) = {
+    var result,br;
+    result <- witness;
+    br <- false;
+    (result,br) <- whp(1,na,false,result);
+    return result;
+  }
+  
+  proc main(n : int) = {
+    var r,c : int;
+    var b : bool;
+    r <- witness;
+    c <- 1;
+    b <- false;
+    while(c <= n /\ !b ){
+     r <$ myd;
+     b <$ {0,1};      
+     c <- c + 1;
+    }
+    return r;
+  }  
+}.
+
+lemma kk : equiv [M.main ~ M.main' : ={arg} ==> ={res}].
+proof. proc. 
+inline*.
+sp. wp.
+while (={c,b,r,n}).
+wp. 
+rnd. rnd. skip.  progress. skip. progress.
+qed.
+
+
+lemma qq : equiv [M.main' ~ M.main'_split : ={arg} ==> ={res}].
+proof. proc.
+sp. inline*. sp.
+unroll {1} 1.
+if. progress.
+wp.
+seq 3 7 : (={r,c,b,n}).
+wp.  rnd. rnd. skip. progress. sim.
+sp.
+rcondf {1} 1. progress. 
+rcondf {2} 1. progress.  skip. progress. smt. wp.  skip. smt.
+qed.
+
+
+
+lemma zqq o (P : _ -> bool) : 0 <= o
+    => equiv [M.whp ~ M.whp : c{1} = c{2} + o /\ n{1} = n{2} + o /\ ={b,r}  ==> (P res{1}) = P res{2}].
+proof. move => oass. proc. 
+inline*.
+sp. wp.
+while (c{1} = c{2} + o /\ n{1} = n{2} + o /\ ={b,r}).
+wp. rnd. rnd. skip. progress. smt. smt.  smt.
+skip. progress. smt. smt.
+qed.
+
+
+lemma zzt &m P : forall np r, 0 < np =>
+    Pr[ M.main'_split(np) @ &m : P res ] = Pr[ M.whp(1,np,false,r) @ &m : P res.`1 ].
+proof. progress.
+byequiv. proc. 
+inline*. sp.
+unroll {2} 1.
+wp.  if. smt. 
+while (={c,b,r,n}). wp. rnd. rnd. skip. progress. wp. 
+rnd. rnd. skip. progress. sp. 
+while (={c,b,r,n}). wp. rnd. rnd. skip.  progress. skip. progress.
+smt. auto. auto.
+qed.
+
+
+lemma okk &m ca na ba ra P : 
+ phoare[ M.whp : arg = (ca,na,ba,ra) ==> P res] =  Pr[M.whp(ca,na,ba,ra) @ &m : P res].
+proof. bypr.
+progress.
+byequiv (_: ={arg} ==> _).
+proc.  while (={c,n,b,r}). wp. rnd. rnd. skip. progress. skip. progress. 
+smt.
+auto.
+qed.
+
+lemma zz &m P : forall np, 0 < np => Pr[ M.main'_split(np) @ &m : P res ] = mu myd P.
+proof.  apply ge0ind.
+simplify. smt.
+simplify. auto.
+simplify. move => np. progress.
+case (np = 0).
+move => np0. rewrite np0. simplify.
+byphoare (_: na = 1 ==> _).
+  proc. sp.
+rcondt 1.
+skip.  auto. inline*.
+rcondf 8.
+wp.  rnd. rnd. skip. progress. 
+wp. rnd. rnd. skip. smt.
+  auto. auto.
+move => p1.
+have : 0 < np. smt.
+clear p1. clear H1.
+move => npe.
+have : Pr[M.main'_split(np) @ &m : P res] = mu myd P.
+apply H0. auto.
+clear H0 H.
+move => ih.
+byphoare (_: na = np+1 ==> _). 
+proc.  sp.
+rcondt 1. skip.  smt.
+swap 2 -1.
+seq 1 : (ca = 1  /\ na = np + 1) (1%r) (mu myd P) (0%r) (1%r).
+rnd. skip. smt.
+rnd. skip. progress. smt.
+case (ba = true).
+inline*.
+rcondf 7. wp.  rnd. skip. progress. wp.
+rnd. skip. smt.
+seq 2 : (na = np + 1 /\ ba = false) (1%r) (mu myd P) (0%r) (1%r).
+wp. rnd. skip. auto.
+wp. rnd. skip. progress.  smt. admit.
+rewrite (zzt &m P np witness) in ih.
+  auto.
+exists* result. elim*. move => r.
+have : Pr[M.whp(2, np + 1, false, witness) @ &m : P res.`1] = Pr[M.whp(1, np, false, witness) @ &m : P res.`1]. 
+byequiv. proc*.
+ call (zqq 1 (fun (x : int * bool) => P x.`1)).
+skip. progress. smt. smt.  auto. auto.
+have ->: Pr[M.whp(2, np + 1, false, witness) @ &m : P res.`1] =  Pr[M.whp(2, np + 1, false, r) @ &m : P res.`1].
+byequiv. proc. unroll {1} 1. unroll {2} 1.
+seq 1 1 : (={c,n,b,r}). 
+rcondt {1} 1. auto. smt.
+rcondt {2} 1. auto. smt.
+wp. rnd. rnd. skip. progress.
+conseq (_: _ ==> ={c,n,b,r}). auto. sim. auto. auto.
+auto.
+have : Pr[M.whp(2, np + 1, false, r) @ &m : P res.`1] = mu myd P.
+rewrite - ih. apply H. progress.
+clear H ih.
+have : phoare[ M.whp : arg = (2, np+1, false, r) ==> P res.`1] = (mu myd P).
+rewrite -  H0.
+apply (okk &m 2 (np + 1) false r (fun (x : int * bool) => P x.`1)). auto.
+call H. skip.  progress. 
+hoare. wp. rnd. skip. progress. smt. auto.
+hoare. simplify.
+rnd. skip.  progress. auto. auto. auto.
+qed.
+
+
+lemma kl : Pr[ M.main'_split(np) @ &m : b = false ] <= ?
+lemma kl : Pr[ M.main'_split(np) @ &m : b = false /\ P res ] <= ?
+          
+
+lemma kl : Pr[ M.main'_split(np) @ &m : P res /\ b = false ]
+ = (int 2%r) ^ n * Pr[ M.main'_split(np) @ &m : P res ]
